Update before trying to define AccJoin

examples/self-fold/find-a-pair-ex1.dfy
@@ -1,26 +1,34 @@
 /*
 Example for proving equivalence of a self-fold and an iterative solution for 
 the "finding a pair satisfying a predicate" problem. 
-Here we use a simple predicate on integers: p(a, b) iff (b != 0 && a != b && a % b == 0). 
+Here we use a simple predicate on integers that checks for divisibility, 
+but it is commutative. 
 */
 
 include "../lists/list-utils.dfy"
 module FindAPair1 {
   import opened Lists 
 
+  // The type of the fold state
+  type D = (List, int, bool)
+
+  // Note that p is commutative
   predicate method p(a: int, b: int)
   {
-    b != 0 && a != b && a % b == 0
+    a != b && (a != 0 && b != 0) && 
+    ((b != 0 && a % b == 0) || (a != 0 && b % a == 0))
   }
 
   /**** Naive iterative approach ****/
-  function method Main1(l: List): bool 
+  // Note that we lift this function from the original implementation.
+  function method Main1(l: List): D 
   {
-    F1(l)
+    // The integer doesn't really matter
+    (l, 0, F1(l))
   }
 
   // Outer loop 
-  function method F1(l: List): bool 
+  function method F1(l: List): bool
   {
     match l 
     case Nil => false 
@@ -32,13 +40,13 @@ module FindAPair1 {
   {
     match l 
     case Nil => false 
+    // We modified this a bit since p isn't commutative. 
     case Cons(hd, tl) => p(a, hd) || G1(a, tl)
   }
 
 
   /**** Self-fold approach ****/
-  // The type of the fold state
-  type D = (List, int, bool)
+  
   // Starting value for the outer fold
   const s_0 := (Nil, 0, false);
 
@@ -51,17 +59,19 @@ module FindAPair1 {
   // Postprocessing after the inner fold
   function method post(t: D, a: int): D 
   {
-    // The only things that matter now are the .0 and .2 fields
-    (ListConc(t.0, Cons(a, Nil)), a, t.2 || p(a, a))
+    // The only things that matter now are the .0 and .2 fields.
+    // Hence I set the .1 field to 0 for convenience.
+    (ListConc(t.0, Cons(a, Nil)), 0, t.2 || p(a, a))
   }
 
   // Inner fold operation 
   function method CheckPredicate(t: D, e: int): D 
   {
-    if t.2 then t else (t.0, t.1, p(t.1, e) || p(e, t.1))
+    // p is commutative so we only check once
+    if t.2 then t else (t.0, t.1, p(t.1, e))
   }
 
-  function method Main2(l: List): bool 
+  function method Main2(l: List): D 
   {
     F2(s_0, l)
   }
@@ -101,28 +111,31 @@ module FindAPair1 {
   lemma AccJoinBehaviour(s: D, l: List) 
     ensures F2(s, l) == AccJoin(s, Main2(l))
   {
-
+    assume F2(s, l) == AccJoin(s, Main2(l));
   }
 
-
-
-
-
-
-
+  // We generated this automatically
+  lemma InductiveFact(a: int, tl: List)
+    ensures Main1(Cons(a, tl)) == AccJoin(CheckAll(s_0, a), Main1(tl))
+  {
+    assume Main1(Cons(a, tl)) == AccJoin(CheckAll(s_0, a), Main1(tl));
+  }
 
   lemma EquivalentSchemes(l: List)
-    ensures Main1(l) == Main2(l).2
+    ensures Main1(l).2 == Main2(l).2
   {
     match l 
     case Nil => {}
     case Cons(a, tl) => {
-      EquivalentSchemes(tl);
+      // Same template as that discussed in the Overleaf document
+      var s := CheckAll(s_0, a);
+      AccJoinBehaviour(s, tl);
+      InductiveFact(a, tl);
     }
   }
 
   method Main() {
-    var l := Cons(4, Cons(7, Cons(3, Nil)));
+    var l := Cons(14, Cons(7, Cons(21, Nil)));
     print Main1(l);
     print "\n";
     print Main2(l);
